Prove evaluate_v_ok in most cases
Re-introduce safe_exp and safe_dec predicates, and state and prove
all cases of evaluate_v_ok except for do_app and do_eval.

candle/prover/abstypeScript.sml
@@ -15,12 +15,62 @@ val _ = set_grammar_ancestry [
   "semanticPrimitivesProps", "misc"];
 
 (* -------------------------------------------------------------------------
+ * Expressions are safe if they do not construct anything with a name from the
+ * kernel type constructors (i.e. one of TYPE, TERM, THM), and if they do not
+ * write to the kernel ffi channel.
  *
+ * We can't keep track on whether or not the constructors have been brought
+ * into scope (i.e., by 'open Kernel;'), so we just forbid their short names
+ * everywhere.
  * ------------------------------------------------------------------------- *)
 
 Definition safe_exp_def:
-  safe_exp (x: exp) = T
+  safe_exp = every_exp $ λx.
+               case x of
+                  Con opt xs => ∀id. opt = SOME id ⇒ id_to_n id ∉ kernel_ctors
+                | App op xs => op ≠ FFI kernel_ffi
+                | _ => T
 End
+
+Theorem safe_exp_simps[simp] =
+   [“safe_exp (Raise e)”,
+    “safe_exp (Handle e pes)”,
+    “safe_exp (Lit lit)”,
+    “safe_exp (Con opt xs)”,
+    “safe_exp (Var n)”,
+    “safe_exp (Fun n x)”,
+    “safe_exp (App op xs)”,
+    “safe_exp (Log lop x y)”,
+    “safe_exp (If x y z)”,
+    “safe_exp (Mat e pes)”,
+    “safe_exp (Let opt x y)”,
+    “safe_exp (Letrec f x)”,
+    “safe_exp (Tannot e t)”,
+    “safe_exp (Lannot e l)”]
+  |> map (SIMP_CONV (srw_ss()) [safe_exp_def])
+  |> map (SIMP_RULE (srw_ss()) [GSYM safe_exp_def, SF ETA_ss])
+  |> LIST_CONJ;
+
+Definition safe_dec_def:
+  safe_dec = every_dec $ λd.
+               case d of
+                 Dlet locs pat x => safe_exp x
+               | Dletrec locs funs => EVERY safe_exp (MAP (SND o SND) funs)
+               | _ => T
+End
+
+Theorem safe_dec_simps[simp] =
+  [“safe_dec (Dlet l p x)”,
+   “safe_dec (Dletrec l f)”,
+   “safe_dec (Dtype l tds)”,
+   “safe_dec (Dtabbrev l ns n t)”,
+   “safe_dec (Dexn l n ts)”,
+   “safe_dec (Dmod mn ds)”,
+   “safe_dec (Dlocal ds1 ds2)”,
+   “safe_dec (Denv n)”]
+  |> map (SIMP_CONV (srw_ss()) [safe_dec_def])
+  |> map (SIMP_RULE (srw_ss()) [GSYM safe_dec_def, SF ETA_ss])
+  |> LIST_CONJ;
 
 Inductive v_ok:
 [~Inferred:]
@@ -75,6 +125,19 @@ Inductive v_ok:
        env_ok ctxt env)
 End
 
+Theorem v_ok_def =
+  [“v_ok ctxt (Conv opt vs)”,
+   “v_ok ctxt (Closure env n x)”,
+   “v_ok ctxt (Recclosure env f n)”,
+   “v_ok ctxt (Vectorv vs)”,
+   “v_ok ctxt (Litv lit)”,
+   “v_ok ctxt (Loc loc)”,
+   “v_ok ctxt (Env env ns)”]
+  |> map (SIMP_CONV (srw_ss()) [Once v_ok_cases])
+  |> LIST_CONJ;
+
+Theorem env_ok_def = SIMP_CONV (srw_ss()) [Once v_ok_cases] “env_ok ctxt env”;
+
 Definition ref_ok_def:
   ref_ok ctxt (Varray vs) = EVERY (v_ok ctxt) vs ∧
   ref_ok ctxt (Refv v) = v_ok ctxt v ∧
@@ -98,8 +161,9 @@ Theorem env_ok_write_cons:
   env_ok ctxt env ⇒
     env_ok ctxt (write_cons nm (n, TypeStamp s t) env)
 Proof
-  rw [Once v_ok_cases]
-  \\ simp [Once v_ok_cases, ml_progTheory.nsLookup_write_cons, SF SFY_ss]
+  simp [env_ok_def]
+  \\ strip_tac
+  \\ simp [ml_progTheory.nsLookup_write_cons, SF SFY_ss]
   \\ Cases \\ simp [ml_progTheory.nsLookup_write_cons]
   \\ rw [] \\ gs [SF SFY_ss]
 QED
@@ -109,8 +173,9 @@ Theorem env_ok_write:
   v_ok ctxt v ⇒
     env_ok ctxt (write nm v env)
 Proof
-  rw [Once v_ok_cases]
-  \\ simp [Once v_ok_cases, ml_progTheory.nsLookup_write, SF SFY_ss]
+  simp [env_ok_def]
+  \\ strip_tac
+  \\ simp [ml_progTheory.nsLookup_write, SF SFY_ss]
   \\ Cases \\ simp [ml_progTheory.nsLookup_write]
   \\ rw [] \\ gs [SF SFY_ss]
 QED
@@ -120,10 +185,9 @@ Theorem env_ok_merge_env:
   env_ok ctxt env2 ⇒
     env_ok ctxt (merge_env env1 env2)
 Proof
-  simp [GSYM AND_IMP_INTRO]
-  \\ simp [Once v_ok_cases] \\ strip_tac
-  \\ simp [Once v_ok_cases] \\ strip_tac
-  \\ simp [Once v_ok_cases, ml_progTheory.merge_env_def]
+  simp [env_ok_def]
+  \\ strip_tac
+  \\ simp [ml_progTheory.merge_env_def]
   \\ conj_tac
   \\ Cases \\ gs [nsLookup_nsAppend_some, SF SFY_ss]
   \\ rw [] \\ gs [SF SFY_ss]
@@ -133,8 +197,7 @@ Theorem env_ok_with:
   env_ok ctxt (env1 with c := env.c) ⇒
     env_ok ctxt (env with v := env1.v)
 Proof
-  rw [Once v_ok_cases]
-  \\ simp [Once v_ok_cases, SF SFY_ss]
+  rw [env_ok_def]
 QED
 
 Theorem env_ok_with_nsBind:
@@ -142,10 +205,8 @@ Theorem env_ok_with_nsBind:
   env_ok ctxt (env2 with c := env.c) ⇒
     env_ok ctxt (env with v := nsBind n v env2.v )
 Proof
-  simp [GSYM AND_IMP_INTRO]
+  simp [env_ok_def]
   \\ strip_tac
-  \\ rw [Once v_ok_cases]
-  \\ simp [Once v_ok_cases]
   \\ conj_tac
   \\ Cases \\ simp [ml_progTheory.nsLookup_nsBind_compute]
   \\ rw [] \\ gs [SF SFY_ss]
@@ -154,7 +215,7 @@ QED
 Theorem env_ok_empty_env:
   env_ok ctxt empty_env
 Proof
-  rw [Once v_ok_cases, ml_progTheory.empty_env_def]
+  rw [env_ok_def, ml_progTheory.empty_env_def]
 QED
 
 (*
@@ -164,7 +225,7 @@ QED
 Theorem env_ok_init_env:
   env_ok ctxt init_env
 Proof
-  rw [Once v_ok_cases, ml_progTheory.init_env_def]
+  rw [env_ok_def, ml_progTheory.init_env_def]
   \\ gvs [nsLookup_Bind_v_some, CaseEqs ["bool", "option"], kernel_types_def]
 QED
 
@@ -185,7 +246,6 @@ Proof
   \\ irule v_ok_Recclosure
   \\ simp [env_ok_merge_env, env_ok_kernel_env, perms_ok_exp_def,
            env_ok_init_env]
-  \\ cheat (* FIXME: Define safe_exp *)
 QED
 
 (* TODO: Use v_thms *)
@@ -280,6 +340,7 @@ Theorem Arrow2:
   A a av ∧ B b bv ∧
   DoEval ∉ ps ∧
   RefAlloc ∉ ps ∧
+  W8Alloc ∉ ps ∧
   (∀n. RefMention n ∉ ps) ∧
   perms_ok ps av ∧
   perms_ok ps bv ∧
@@ -296,7 +357,8 @@ Proof
   \\ ‘LENGTH s'.refs = LENGTH s.refs’
     by (gvs [do_partial_app_def, CaseEqs ["v", "exp"], do_opapp_cases,
              perms_ok_def]
-        \\ drule_at_then (Pos (el 5)) (qspec_then ‘ps’ mp_tac)
+        \\ drule_at_then (Pat ‘evaluate’)
+                         (qspec_then ‘ps’ mp_tac)
                          evaluate_perms_ok_exp
         \\ impl_tac \\ simp []
         \\ gs [perms_ok_state_def, perms_ok_env_def]
@@ -349,7 +411,7 @@ Proof
   >- (
     irule TERM_from_TERM_TYPE
     \\ gs [SF SFY_ss])
-  \\ Cases_on ‘tm’ \\ gvs [TERM_TYPE_def, Once v_ok_cases, kernel_types_def]
+  \\ Cases_on ‘tm’ \\ gvs [TERM_TYPE_def, v_ok_def, kernel_types_def]
   \\ gvs [Once v_ok_cases, do_partial_app_def, CaseEqs ["exp", "v"]]
 QED
 
@@ -363,14 +425,14 @@ Proof
   >- (
     irule THM_from_THM_TYPE
     \\ gs [SF SFY_ss])
-  \\ Cases_on ‘th’ \\ gvs [THM_TYPE_def, Once v_ok_cases, kernel_types_def]
+  \\ Cases_on ‘th’ \\ gvs [THM_TYPE_def, v_ok_def, kernel_types_def]
   \\ gvs [Once v_ok_cases, do_partial_app_def, CaseEqs ["exp", "v"]]
 QED
 
 Theorem v_ok_bind_exn_v[simp]:
   v_ok ctxt bind_exn_v
 Proof
-  rw [Once v_ok_cases, bind_exn_v_def]
+  rw [v_ok_def, bind_exn_v_def]
   \\rw [Once v_ok_cases, bind_stamp_def, kernel_types_def]
 QED
 
@@ -501,6 +563,7 @@ Proof
       \\ assume_tac conj_v_thm
       \\ ‘∃ps. DoEval ∉ ps ∧
                RefAlloc ∉ ps ∧
+               W8Alloc ∉ ps ∧
                (∀n. RefMention n ∉ ps) ∧
                perms_ok ps conj_v’
         by (irule_at Any conj_v_perms_ok
@@ -528,6 +591,7 @@ Proof
       \\ assume_tac disj1_v_thm
       \\ ‘∃ps. DoEval ∉ ps ∧
                RefAlloc ∉ ps ∧
+               W8Alloc ∉ ps ∧
                (∀n. RefMention n ∉ ps) ∧
                perms_ok ps disj1_v’
         by (irule_at Any disj1_v_perms_ok
@@ -562,6 +626,8 @@ Proof
     \\ rw [kernel_funs_def])
 QED
 
+(* TODO Why is everything named compile_xxx? *)
+
 local
   val ind_thm =
     full_evaluate_ind
@@ -585,6 +651,8 @@ local
         evaluate_match s env v ps errv = (s', res) ∧
         state_ok ctxt s ∧
         env_ok ctxt env ∧
+        v_ok ctxt v ∧
+        v_ok ctxt errv ∧
         EVERY safe_exp (MAP SND ps) ⇒
           ∃ctxt'.
             (∀v. v_ok ctxt v ⇒ v_ok ctxt' v) ∧
@@ -600,13 +668,13 @@ local
         evaluate_decs s env ds = (s', res) ∧
         state_ok ctxt s ∧
         env_ok ctxt env ∧
-        EVERY safe_exp (MAP SND ps) ⇒
+        EVERY safe_dec ds ⇒
           ∃ctxt'.
             (∀v. v_ok ctxt v ⇒ v_ok ctxt' v) ∧
             case res of
-              Rval env =>
+              Rval env1 =>
                 state_ok ctxt' s'  ∧
-                env_ok ctxt env
+                env_ok ctxt' (extend_dec_env env1 env)
             | Rerr (Rraise v) =>
                 state_ok ctxt' s'  ∧
                 v_ok ctxt' v
@@ -636,10 +704,7 @@ Proof
   \\ drule_then strip_assume_tac evaluate_sing \\ gvs []
   \\ first_x_assum (drule_all_then (qx_choose_then ‘ctxt1’ assume_tac)) \\ gs []
   \\ ‘env_ok ctxt1 env’
-    by (qpat_x_assum ‘env_ok _ _’ mp_tac
-        \\ rw [Once v_ok_cases]
-        \\ rw [Once v_ok_cases]
-        \\ gs [SF SFY_ss])
+    by gs [env_ok_def, SF SFY_ss]
   \\ first_x_assum (drule_all_then strip_assume_tac) \\ gs []
   \\ rpt CASE_TAC \\ gs []
   \\ gs [state_ok_def]
@@ -659,8 +724,7 @@ Theorem compile_Raise:
 Proof
   rw [evaluate_def] \\ gs []
   \\ gvs [CaseEqs ["result", "prod"]]
-  \\ cheat (* FIXME: Define safe_exp *) (*
-  \\ drule_then strip_assume_tac evaluate_sing \\ gvs [] *)
+  \\ drule_then strip_assume_tac evaluate_sing \\ gvs []
 QED
 
 Theorem compile_Handle:
@@ -668,18 +732,14 @@ Theorem compile_Handle:
 Proof
   rw [evaluate_def]
   \\ gvs [CaseEqs ["result", "prod", "error_result", "bool"], EVERY_MAP]
-  \\ cheat (* FIXME: Define safe_exp *) (*
   \\ first_x_assum (drule_all_then (qx_choose_then ‘ctxt1’ assume_tac)) \\ gs []
   >~ [‘¬can_pmatch_all _ _ _ _’] >- (
     gs [state_ok_def]
     \\ first_assum (irule_at Any) \\ gs [])
   \\ ‘env_ok ctxt1 env’
-    by (qpat_x_assum ‘env_ok _ _’ mp_tac
-        \\ rw [Once v_ok_cases]
-        \\ rw [Once v_ok_cases]
-        \\ gs [SF SFY_ss])
+    by gs [env_ok_def, SF SFY_ss]
   \\ first_x_assum (drule_all_then strip_assume_tac)
-  \\ first_assum (irule_at Any) \\ gs [] *)
+  \\ first_assum (irule_at Any) \\ gs []
 QED
 
 Theorem compile_Con:
@@ -687,7 +747,6 @@ Theorem compile_Con:
 Proof
   rw [evaluate_def]
   \\ gvs [CaseEqs ["result", "prod", "error_result", "option"], EVERY_MAP]
-  \\ cheat (* FIXME: Define safe_exp *) (*
   >~ [‘¬do_con_check _ _ _’] >- (
     gs [state_ok_def]
     \\ first_assum (irule_at Any) \\ gs [])
@@ -698,9 +757,8 @@ Proof
   \\ first_x_assum (drule_all_then (qx_choose_then ‘ctxt1’ assume_tac)) \\ gs []
   \\ first_assum (irule_at Any) \\ gs []
   \\ gvs [build_conv_def, CaseEqs ["option", "prod"]]
-  \\ irule v_ok_Conv \\ gs []
-  \\ qpat_x_assum ‘env_ok _ _’ mp_tac
-  \\ rw [Once v_ok_cases] \\ gs [SF SFY_ss] *)
+  \\ irule v_ok_Conv \\ gs [] \\ rw []
+  \\ gs [env_ok_def, SF SFY_ss]
 QED
 
 Theorem compile_Var:
@@ -711,9 +769,8 @@ Proof
   >- (
     gs [state_ok_def]
     \\ metis_tac [])
-  \\ first_assum (irule_at Any) \\ gs []
-  \\ qpat_x_assum ‘env_ok _ _’ mp_tac
-  \\ rw [Once v_ok_cases] \\ gs [SF SFY_ss]
+  \\ first_assum (irule_at Any)
+  \\ gs [env_ok_def, SF SFY_ss]
 QED
 
 Theorem compile_Fun:
@@ -721,10 +778,8 @@ Theorem compile_Fun:
 Proof
   rw [evaluate_def]
   \\ gvs [CaseEqs ["option"]]
-  \\ cheat (* FIXME: Define safe_exp *) (*
   \\ first_assum (irule_at Any) \\ gs []
   \\ irule v_ok_Closure \\ gs []
-  \\ first_assum (irule_at Any) *)
 QED
 
 Theorem compile_App:
@@ -732,7 +787,6 @@ Theorem compile_App:
 Proof
   rw [evaluate_def]
   \\ gvs [CaseEqs ["prod", "result", "option", "error_result", "bool"]]
-  \\ cheat (* FIXME: Define safe_exp *) (*
   >~ [‘do_opapp _ = NONE’] >- (
     first_x_assum (drule_all_then strip_assume_tac)
     \\ gs [state_ok_def]
@@ -743,10 +797,7 @@ Proof
     \\ first_assum (irule_at Any) \\ gs [])
   \\ first_x_assum (drule_all_then (qx_choose_then ‘ctxt1’ assume_tac)) \\ gs []
   \\ ‘env_ok ctxt1 env’
-    by (qpat_x_assum ‘env_ok _ _’ mp_tac
-        \\ rw [Once v_ok_cases]
-        \\ rw [Once v_ok_cases]
-        \\ gs [SF SFY_ss])
+    by gs [env_ok_def, SF SFY_ss]
   \\ rename1 ‘state_ok ctxt1 s’
   \\ ‘state_ok ctxt1 (dec_clock s)’
     by gs [evaluateTheory.dec_clock_def, state_ok_def]
@@ -767,50 +818,372 @@ Proof
     \\ CASE_TAC \\ gs []
     \\ gs [state_ok_def])
   \\ rename1 ‘do_opapp _ = SOME (env1, e)’
-  \\ ‘env_ok ctxt1 env1’
-    by (gvs [do_opapp_cases]
-        >~ [‘Closure env1 n e’] >- (
-          irule env_ok_with_nsBind \\ gs []
-          \\ ‘env1 with c := env1.c = env1’
-            by rw [sem_env_component_equality]
-          \\ gs []
-          \\ qpat_x_assum ‘v_ok _ (Closure _ _ _)’ mp_tac
-          \\ rewrite_tac [Once v_ok_cases] \\ simp []
-          \\ rw [] \\ gs [])
-        \\ qpat_x_assum ‘v_ok _ (Recclosure _ _ _)’ mp_tac
-        \\ rewrite_tac [Once v_ok_cases] \\ simp []
-        \\ rw [Once v_ok_cases]
-        \\ simp [Once v_ok_cases, SF SFY_ss]
-        \\ Cases \\ simp [build_rec_env_merge,
-                          ml_progTheory.nsLookup_nsBind_compute]
-        \\ rw [] \\ gs []
-        \\ gs [nsLookup_nsAppend_some, nsLookup_alist_to_ns_some,
-               nsLookup_alist_to_ns_none]
-        >~ [‘ALOOKUP _ _ = SOME _’] >- (
-          drule_then assume_tac ALOOKUP_MEM
-          \\ gvs [MEM_MAP, EXISTS_PROD]
-          \\ rewrite_tac [Once v_ok_cases] \\ simp []
-          \\ rw [DISJ_EQ_IMP]
-          \\ gs [EVERY_MAP, EVERY_MEM, FORALL_PROD, SF SFY_ss]
-          \\ simp [Once v_ok_cases, SF SFY_ss]
-          \\ first_assum (irule_at Any) \\ gs []
-          \\ rw []
-          \\ first_x_assum irule
-          \\ gs [SF SFY_ss])
-        \\ first_x_assum irule
-        \\ gs [SF SFY_ss])
-  \\ cheat (* there's permissions in v_ok now *) *)
+  \\ ‘env_ok ctxt1 env1 ∧ safe_exp e’
+    suffices_by (
+      strip_tac
+      \\ last_x_assum (drule_all_then strip_assume_tac)
+      \\ qexists_tac ‘ctxt'’
+      \\ gs [evaluateTheory.dec_clock_def, state_ok_def, EVERY_MEM,
+             AC CONJ_COMM CONJ_ASSOC])
+  \\ gvs [v_ok_def, state_ok_def, do_opapp_cases]
+  >~ [‘Closure env1 n e’] >- (
+    irule env_ok_with_nsBind \\ gs []
+    \\ ‘env1 with c := env1.c = env1’
+      by rw [sem_env_component_equality]
+    \\ gs [])
+  \\ gs [env_ok_def, evaluateTheory.dec_clock_def, find_recfun_ALOOKUP,
+         SF SFY_ss]
+  \\ drule_then assume_tac ALOOKUP_MEM
+  \\ gs [EVERY_MEM, EVERY_MAP, FORALL_PROD, SF SFY_ss]
+  \\ Cases \\ simp [build_rec_env_merge, ml_progTheory.nsLookup_nsBind_compute]
+  \\ rw [] \\ gs []
+  \\ gs [nsLookup_nsAppend_some, nsLookup_alist_to_ns_some,
+         nsLookup_alist_to_ns_none]
+  >~ [‘ALOOKUP _ _ = SOME _’] >- (
+    drule_then assume_tac ALOOKUP_MEM
+    \\ gvs [MEM_MAP, EXISTS_PROD, v_ok_def, EVERY_MEM]
+    \\ rw [DISJ_EQ_IMP, env_ok_def] \\ gs [SF SFY_ss])
+  \\ first_x_assum irule
+  \\ gs [SF SFY_ss]
+QED
+
+Theorem compile_Log:
+  ^(get_goal "Log")
+Proof
+  rw [evaluate_def]
+  \\ gvs [CaseEqs ["prod", "result", "option", "error_result", "exp_or_val",
+                   "bool"], do_log_def]
+  \\ drule_then strip_assume_tac evaluate_sing \\ gvs []
+  >- (
+    first_x_assum (drule_all_then strip_assume_tac)
+    \\ gs [state_ok_def]
+    \\ first_assum (irule_at Any) \\ gs [])
+  \\ first_x_assum (drule_all_then strip_assume_tac)
+  \\ rename1 ‘v_ok ctxt1 (Boolv _)’
+  \\ ‘env_ok ctxt1 env’
+    suffices_by (
+      strip_tac
+      \\ first_x_assum (drule_all_then strip_assume_tac)
+      \\ first_assum (irule_at Any) \\ gs [])
+  \\ gs [env_ok_def, SF SFY_ss]
+QED
+
+Theorem compile_If:
+  ^(get_goal "If")
+Proof
+  rw [evaluate_def]
+  \\ gvs [CaseEqs ["prod", "result", "option", "error_result", "exp_or_val",
+                   "bool"], do_if_def]
+  \\ drule_then strip_assume_tac evaluate_sing \\ gvs []
+  >- (
+    first_x_assum (drule_all_then strip_assume_tac)
+    \\ gs [state_ok_def]
+    \\ first_assum (irule_at Any) \\ gs [])
+  \\ first_x_assum (drule_all_then strip_assume_tac)
+  \\ rename1 ‘v_ok ctxt1 (Boolv _)’
+  \\ ‘env_ok ctxt1 env’
+    suffices_by (
+      strip_tac
+      \\ first_x_assum (drule_all_then strip_assume_tac)
+      \\ first_assum (irule_at Any) \\ gs [])
+  \\ gs [env_ok_def, SF SFY_ss]
+QED
+
+Theorem compile_Mat:
+  ^(get_goal "Mat")
+Proof
+  rw [evaluate_def]
+  \\ gvs [CaseEqs ["prod", "result", "option", "error_result", "bool"]]
+  \\ drule_then strip_assume_tac evaluate_sing \\ gvs []
+  \\ first_x_assum (drule_all_then strip_assume_tac)
+  >~ [‘¬can_pmatch_all _ _ _ _’] >- (
+    gs [state_ok_def]
+    \\ first_assum (irule_at Any) \\ gs [])
+  \\ rename1 ‘v_ok ctxt1 v’
+  \\ ‘env_ok ctxt1 env’
+    suffices_by (
+      strip_tac
+      \\ first_x_assum (drule_all_then strip_assume_tac)
+      \\ first_assum (irule_at Any) \\ gs [])
+  \\ gs [env_ok_def, SF SFY_ss]
+QED
+
+Theorem compile_Let:
+  ^(get_goal "Let")
+Proof
+  rw [evaluate_def]
+  \\ gvs [CaseEqs ["prod", "result", "option", "error_result"]]
+  \\ first_x_assum (drule_all_then strip_assume_tac) \\ gs []
+  \\ drule_then strip_assume_tac evaluate_sing \\ gvs []
+  \\ rename1 ‘v_ok ctxt1 v’
+  \\ ‘env_ok ctxt1 (env with v := nsOptBind xo v env.v)’
+    suffices_by (
+      strip_tac
+      \\ first_x_assum (drule_all_then strip_assume_tac)
+      \\ first_assum (irule_at Any)
+      \\ gs [])
+  \\ gs [env_ok_def, SF SFY_ss]
+  \\ Cases_on ‘xo’ \\ gs [namespaceTheory.nsOptBind_def, SF SFY_ss]
+  \\ Cases \\ simp [ml_progTheory.nsLookup_nsBind_compute]
+  \\ rw [] \\ gs [SF SFY_ss]
+QED
+
+Theorem compile_Letrec:
+  ^(get_goal "Letrec")
+Proof
+  rw [evaluate_def]
+  \\ gvs [CaseEqs ["prod", "result", "option", "error_result"]]
+  >~ [‘¬ALL_DISTINCT _’] >- (
+    gs [state_ok_def]
+    \\ first_assum (irule_at Any) \\ gs [])
+  \\ ‘env_ok ctxt (env with v := build_rec_env funs env env.v)’
+    suffices_by (
+      strip_tac
+      \\ first_x_assum (drule_all_then strip_assume_tac)
+      \\ first_assum (irule_at Any) \\ gs [])
+  \\ gs [env_ok_def, SF SFY_ss]
+  \\ simp [build_rec_env_merge, nsLookup_nsAppend_some,
+           nsLookup_alist_to_ns_some,
+           nsLookup_alist_to_ns_none]
+  \\ rw [] \\ gs [SF SFY_ss]
+  \\ drule_then assume_tac ALOOKUP_MEM
+  \\ gvs [MEM_MAP, EXISTS_PROD, PULL_EXISTS, v_ok_def]
+  \\ rw [DISJ_EQ_IMP, env_ok_def] \\ gs [SF SFY_ss]
+QED
+
+Theorem compile_Tannot:
+  ^(get_goal "Tannot")
+Proof
+  rw [evaluate_def]
+QED
+
+Theorem compile_Lannot:
+  ^(get_goal "Lannot")
+Proof
+  rw [evaluate_def]
+QED
+
+Theorem compile_pmatch_Nil:
+  ^(get_goal "[]:(pat # exp) list")
+Proof
+  rw [evaluate_def] \\ gs []
+  \\ first_assum (irule_at Any) \\ gs []
+QED
+
+Theorem compile_pmatch_Cons:
+  ^(get_goal "_::_:(pat # exp) list")
+Proof
+  rw [evaluate_def] \\ gs []
+  \\ gvs [CaseEqs ["bool", "match_result"]]
+  >~ [‘Match env1’] >- (
+    ‘env_ok ctxt (env with v := nsAppend (alist_to_ns env1) env.v)’
+      suffices_by (
+        strip_tac
+        \\ first_x_assum (drule_all_then strip_assume_tac)
+        \\ first_assum (irule_at Any) \\ gs [])
+    \\ gs [env_ok_def, SF SFY_ss]
+    \\ simp [nsLookup_nsAppend_some, nsLookup_alist_to_ns_some,
+             nsLookup_alist_to_ns_none]
+    \\ rw [] \\ gs [SF SFY_ss]
+    \\ drule_then assume_tac ALOOKUP_MEM
+    \\ cheat (* pmatch theorem *))
+  \\ gs [state_ok_def]
+  \\ first_assum (irule_at Any) \\ gs []
+QED
+
+Theorem compile_decs_Nil:
+  ^(get_goal "[]:dec list")
+Proof
+  rw [evaluate_decs_def, extend_dec_env_def]
+  \\ first_assum (irule_at Any) \\ gs []
+QED
+
+Theorem compile_decs_Cons:
+  ^(get_goal "_::_::_:dec list")
+Proof
+  rw [evaluate_decs_def]
+  \\ gvs [CaseEqs ["prod", "result"]]
+  \\ first_x_assum (drule_all_then strip_assume_tac)
+  \\ rename1 ‘state_ok ctxt1 st1’
+  \\ ‘env_ok ctxt1 (extend_dec_env env1 env)’
+    by gs [extend_dec_env_def, env_ok_def, SF SFY_ss]
+  \\ first_x_assum (drule_all_then strip_assume_tac)
+  \\ gs [state_ok_def, combine_dec_result_def]
+  \\ CASE_TAC \\ gs [AC CONJ_COMM CONJ_ASSOC]
+  >~ [‘Rerr err’] >- (
+    CASE_TAC \\ gs []
+    \\ first_assum (irule_at Any) \\ gs [])
+  \\ first_x_assum (irule_at Any) \\ gs []
+  \\ gs [env_ok_def, extend_dec_env_def, nsLookup_nsAppend_some]
+  \\ rw [] \\ gs [SF SFY_ss]
+QED
+
+Theorem compile_decs_Dlet:
+  ^(get_goal "Dlet")
+Proof
+  rw [evaluate_decs_def]
+  >~ [‘¬ALL_DISTINCT _’] >- (
+    gs [state_ok_def]
+    \\ first_assum (irule_at Any) \\ gs [])
+  \\ gvs [CaseEqs ["prod", "result"]]
+  \\ drule_then strip_assume_tac evaluate_sing \\ gvs []
+  \\ first_x_assum (drule_all_then strip_assume_tac)
+  \\ CASE_TAC \\ gs [state_ok_def]
+  \\ first_assum (irule_at Any) \\ gs []
+  \\ gs [extend_dec_env_def, env_ok_def, nsLookup_nsAppend_some,
+         nsLookup_alist_to_ns_some, SF SFY_ss]
+  \\ rw [] \\ gs [SF SFY_ss]
+  \\ drule_then assume_tac ALOOKUP_MEM
+  \\ cheat (* pmatch theorem *)
+QED
+
+Theorem compile_decs_Dletrec:
+  ^(get_goal "Dletrec")
+Proof
+  rw [evaluate_decs_def]
+  >~ [‘¬ALL_DISTINCT _’] >- (
+    gs [state_ok_def]
+    \\ first_assum (irule_at Any) \\ gs [])
+  \\ gvs [CaseEqs ["prod", "result"]]
+  \\ first_assum (irule_at Any) \\ gs []
+  \\ gs [extend_dec_env_def, build_rec_env_merge, env_ok_def,
+         nsLookup_nsAppend_some, nsLookup_alist_to_ns_some, SF SFY_ss]
+  \\ rw [] \\ gs [SF SFY_ss]
+  \\ drule_then assume_tac ALOOKUP_MEM
+  \\ gvs [MEM_MAP, EXISTS_PROD]
+  \\ simp [v_ok_def, DISJ_EQ_IMP]
+  \\ rw [] \\ gs [env_ok_def, SF SFY_ss]
+QED
+
+Theorem compile_decs_Dtype:
+  ^(get_goal "Dtype")
+Proof
+  rw [evaluate_decs_def]
+  >~ [‘¬EVERY check_dup_ctors _’] >- (
+    gs [state_ok_def]
+    \\ first_assum (irule_at Any) \\ gs [])
+  \\ gvs [CaseEqs ["prod", "result"], state_ok_def]
+  \\ first_assum (irule_at Any) \\ gs []
+  \\ conj_tac
+  >- (
+    rw []
+    \\ first_x_assum drule \\ gs [])
+  \\ gs [extend_dec_env_def, build_tdefs_def, env_ok_def,
+         nsLookup_nsAppend_some, nsLookup_alist_to_ns_some, SF SFY_ss]
+  \\ rw [] \\ gs [SF SFY_ss]
+  \\ ‘∀m tds n l t k.
+        nsLookup (build_tdefs m tds) n = SOME (l, TypeStamp t k) ⇒
+          m ≤ k’
+    by (ho_match_mp_tac build_tdefs_ind
+        \\ simp [build_tdefs_def, nsLookup_nsAppend_some,
+                 nsLookup_alist_to_ns_some, SF SFY_ss]
+        \\ rw [] \\ gs [SF SFY_ss]
+        >- (
+          first_x_assum drule
+          \\ gs [])
+        \\ drule_then assume_tac ALOOKUP_MEM
+        \\ gs [build_constrs_def, MEM_MAP, EXISTS_PROD])
+  \\ first_x_assum (drule_then assume_tac)
+  \\ strip_tac
+  \\ first_x_assum drule_all \\ gs []
+QED
+
+Theorem compile_decs_Dtabbrev:
+  ^(get_goal "Dtabbrev")
+Proof
+  rw [evaluate_decs_def]
+  \\ first_assum (irule_at Any)
+  \\ gs [env_ok_def, extend_dec_env_def, SF SFY_ss]
+QED
+
+Theorem compile_decs_Denv:
+  ^(get_goal "Denv")
+Proof
+  rw [evaluate_decs_def]
+  \\ gvs [CaseEqs ["option", "prod"]]
+  \\ gs [state_ok_def]
+  \\ first_assum (irule_at Any) \\ gs []
+  \\ gs [env_ok_def, extend_dec_env_def, SF SFY_ss]
+  \\ gvs [declare_env_def, CaseEqs ["option", "eval_state", "prod"]]
+  \\ Cases \\ simp [ml_progTheory.nsLookup_nsBind_compute]
+  \\ rw [] \\ gs [v_ok_def, env_ok_def, nat_to_v_def, SF SFY_ss]
+QED
+
+Theorem compile_decs_Dexn:
+  ^(get_goal "Dexn")
+Proof
+  rw [evaluate_decs_def]
+  \\ gvs [CaseEqs ["option", "prod"], state_ok_def]
+  \\ first_assum (irule_at Any) \\ gs []
+  \\ gs [env_ok_def, extend_dec_env_def, SF SFY_ss]
+  \\ Cases \\ simp [ml_progTheory.nsLookup_nsBind_compute]
+  \\ rw [] \\ gs [SF SFY_ss]
+QED
+
+Theorem compile_decs_Dmod:
+  ^(get_goal "Dmod")
+Proof
+  rw [evaluate_decs_def]
+  \\ gvs [CaseEqs ["option", "prod", "result"]]
+  \\ first_x_assum (drule_all_then strip_assume_tac)
+  \\ first_assum (irule_at Any) \\ gs []
+  \\ gs [env_ok_def, extend_dec_env_def, SF SFY_ss]
+  \\ conj_tac
+  \\ Cases \\ gs [ml_progTheory.nsLookup_nsBind_compute,
+                  nsLookup_nsAppend_some,
+                  nsLookup_nsLift]
+  \\ rw [] \\ gs [SF SFY_ss]
+QED
+
+Theorem compile_decs_Dlocal:
+  ^(get_goal "Dlocal")
+Proof
+  rw [evaluate_decs_def]
+  \\ gvs [CaseEqs ["option", "prod", "result"]]
+  \\ first_x_assum (drule_all_then strip_assume_tac)
+  \\ first_x_assum (drule_all_then strip_assume_tac)
+  \\ CASE_TAC \\ gs []
+  \\ first_assum (irule_at Any) \\ gs []
+  \\ gs [env_ok_def, extend_dec_env_def, SF SFY_ss]
+  \\ conj_tac
+  \\ Cases \\ gs [ml_progTheory.nsLookup_nsBind_compute,
+                nsLookup_nsAppend_some]
+  \\ rw [] \\ gs [SF SFY_ss]
 QED
 
 Theorem evaluate_v_ok:
   ^(compile_correct_tm ())
 Proof
   match_mp_tac (the_ind_thm ())
-  \\ rpt conj_tac
-  \\ rewrite_tac [compile_Nil, compile_Cons, compile_Lit, compile_Raise,
-                 compile_Handle, compile_Con, compile_Var, compile_Fun,
-                 compile_App]
-  \\ cheat
+  \\ rpt conj_tac \\ rpt gen_tac
+  >- rewrite_tac [compile_Nil]
+  >- rewrite_tac [compile_Cons]
+  >- rewrite_tac [compile_Lit]
+  >- rewrite_tac [compile_Raise]
+  >- rewrite_tac [compile_Handle]
+  >- rewrite_tac [compile_Con]
+  >- rewrite_tac [compile_Var]
+  >- rewrite_tac [compile_Fun]
+  >- cheat (* App *)
+  >- rewrite_tac [compile_Log]
+  >- rewrite_tac [compile_If]
+  >- rewrite_tac [compile_Mat]
+  >- rewrite_tac [compile_Let]
+  >- rewrite_tac [compile_Letrec]
+  >- rewrite_tac [compile_Tannot]
+  >- rewrite_tac [compile_Lannot]
+  >- rewrite_tac [compile_pmatch_Nil]
+  >- rewrite_tac [compile_pmatch_Cons]
+  >- rewrite_tac [compile_decs_Nil]
+  >- rewrite_tac [compile_decs_Cons]
+  >- rewrite_tac [compile_decs_Dlet]
+  >- rewrite_tac [compile_decs_Dletrec]
+  >- rewrite_tac [compile_decs_Dtype]
+  >- rewrite_tac [compile_decs_Dtabbrev]
+  >- rewrite_tac [compile_decs_Denv]
+  >- rewrite_tac [compile_decs_Dexn]
+  >- rewrite_tac [compile_decs_Dmod]
+  >- rewrite_tac [compile_decs_Dlocal]
 QED
 
 val _ = export_theory ();
